TabularTypeInterpreter/F⊗⊕ω/Semantics/Type/SmallStep.lean
@@ -168,64 +168,17 @@ inductive StronglyNormalizingIn : Nat → «Type» → Prop where
     (sni : (∀ Bn ∈ Bns, StronglyNormalizingIn Bn.snd Bn.fst))
     : StronglyNormalizingIn (Bns.map Prod.snd |>.max?.map (· + 1) |>.getD 0) A
 
-judgement_syntax "SN" K "(" A ")" : IndexedStronglyNormalizing
-
-abbrev IndexedStronglyNormalizing : Kind → «Type» → Prop
-  | [[*]], A => [[ε ⊢ A : *]] ∧ [[SN(A)]]
-  | [[K₁ ↦ K₂]], A => [[ε ⊢ A : K₁ ↦ K₂]] ∧ ∀ B, [[SN K₁ (B)]] → [[SN K₂ (A B)]]
-  | [[L K]], A => [[ε ⊢ A : L K]]
-
-nosubst
-nonterminal Subst, δ :=
-  | "ε"              : empty
-  | δ ", " A " / " a : ext (id a)
-
-namespace Subst
-
-def find? (δ : Subst) (a : TypeVarId) : Option «Type» := match δ with
-  | .empty => none
-  | .ext δ' A a' => if a = a' then A else find? δ' a
-
-def apply (δ : Subst) : «Type» → «Type»
-  | .var a => match a with
-    | .bound n => .var <| .bound n
-    | .free a => if let some A := δ.find? a then
-        A
-      else
-        .var <| .free a
-  | .lam K A => .lam K <| apply δ A
-  | .app A B => .app (apply δ A) (apply δ B)
-  | .forall K A => .forall K <| apply δ A
-  | .arr A B => .arr (apply δ A) (apply δ B)
-  | .list As K? => .list (As.mapMem fun A _ => apply δ A) K?
-  | .listApp A B => .listApp (apply δ A) (apply δ B)
-  | .prod A => .prod <| apply δ A
-  | .sum A => .sum <| apply δ A
-
-instance : CoeFun Subst (fun _ => «Type» → «Type») where
-  coe := Subst.apply
-
-def «dom» : Subst → List TypeVarId
-  | .empty => []
-  | .ext δ _ a => a :: δ.dom
-
-def freeTypeVars : Subst → List TypeVarId
-  | .empty => []
-  | .ext δ A _ => A.freeTypeVars ++ δ.freeTypeVars
-
-end Subst
-
-judgement_syntax δ " ⊨ " Δ : SubstSatisfies
-
-judgement SubstSatisfies := fun (δ : Subst) Δ => δ.dom.Unique ∧ δ.dom = Δ.typeVarDom ∧
-    ∀ a K, [[a : K ∈ Δ]] → IndexedStronglyNormalizing K (δ (Type.var a))
+inductive StronglyNormalizingToList (P : «Type» → Prop) : «Type» → Prop where
+  | refl : (∀ A ∈ As, P A) → StronglyNormalizingToList P (Type.list As K?)
+  | step : (∀ B, [[ε ⊢ A -> B]] → StronglyNormalizingToList P B) → (∀ As K?, A ≠ Type.list As K?) →
+      StronglyNormalizingToList P A
 
 judgement_syntax "neutral " A : Type.Neutral
 
 abbrev Type.Neutral A :=
   (∀ K A', A ≠ [[λ a : K. A']]) ∧
     (∀ A' n K b, A = [[{</ A'@i // i in [:n] /> </ : K // b />}]] → ∀ i ∈ [:n], Neutral (A' i)) ∧
-    ∀ A' B, A = [[A' ⟦B⟧]] → Neutral A' ∧ Neutral B
+    ∀ A' B, A ≠ [[A' ⟦B⟧]]
 termination_by sizeOf A
 decreasing_by
   all_goals (
